coq/NNRC/Core/cNNRC.v
@@ -204,6 +204,8 @@ Section cNNRC.
   Section Top.
     Definition nnrc_core_eval_top (q:nnrc_core) (cenv:bindings) : option data :=
       lift_nnrc_core (nnrc_core_eval (rec_sort (mkConstants cenv))) q.
+    Definition nnrc_core_eval_top_alt (q:nnrc_core) (cenv:bindings) : option data :=
+      lift_nnrc_core (nnrc_core_eval (rec_sort cenv)) q.
   End Top.
   
 End cNNRC.
