coq/NNRC/Core/cNNRCShadow.v
@@ -1751,6 +1751,11 @@ Section cNNRCShadow.
     Qed.
     
   End core.
+
+  Section FreeVars.
+    Fixpoint nnrc_free_variables (q:nnrc) : list var := nnrc_free_vars q.
+  End FreeVars.
+  
 End cNNRCShadow.
 
 (* 
